Update URM.v

URM.v
@@ -1,25 +1,19 @@
 Set Warnings "-notation-overridden,-parsing,-deprecated-hint-without-locality".
-(* From LF Require Export Maps. *)
-Require Import List.
-Require Import Coq.Arith.PeanoNat.
-Require Import Coq.Init.Datatypes.
 Require Import Coq.Lists.List.
 Require Import Coq.Arith.Arith.
 Require Import Lia.
 
 
-Module URM.
     Definition reg := nat -> nat.
-    Definition reg0 : nat -> nat :=
-    (fun _ => 0).
+    Definition reg0 : nat -> nat := (fun _ => 0).
     Lemma reg0_is_correct: forall x : nat, reg0 x = 0.
     Proof. reflexivity. Qed.
-    Definition update_value
-                (f : nat -> nat)(x : nat) (v : nat) :=
-    (fun x' => if Nat.eqb x x' then v else f x').
-    Example fl: forall f: nat -> nat, update_value f 6 5 6 = 5.
-    Proof. reflexivity. Qed.
 
+    Definition update_value (f : nat -> nat)(x : nat) (v : nat) :=
+    (fun x' => if Nat.eqb x x' then v else f x').
+
+    Example fl: forall f: nat -> nat, (update_value f 6 5) 6 = 5.
+    Proof. reflexivity. Qed.
 
     Lemma update_value_is_correct : forall x x' n, forall f, (update_value f x n) x = n /\ ((x=?x') = false -> ((update_value f x n) x' = f x')).
     Proof. split.
@@ -45,7 +39,6 @@ Module URM.
     Notation "x ++ y" := (app x y)
             (right associativity, at level 60).
 
-    Definition Example2_1:= [J 1 2 6;Ss 2;Ss 3;J 1 2 6;J 1 1 2;T 3 1].
     Example ss : length [Z (0);Ss(1);T 2 3] = 3.
      Proof. reflexivity. Qed.
     Example sd : [Z (0)] ++ [Ss(1) ; T 2 3] = [Z (0);Ss(1);T 2 3].
@@ -73,7 +66,6 @@ Module URM.
      Proof. reflexivity. Qed.
     (* others are just as immediate as this one *)
 
-        
 
    Fixpoint execution (p : program) (config : (prod nat (nat -> nat)))  (step : nat) 
    :prod bool (prod nat (nat -> nat)) :=
@@ -91,81 +83,11 @@ Module URM.
     (* note that every computation for a program with another initial config,
       can be sirulated with a program with (1, reg0) config*)
 
-
     Compute (execution [] initial_config 5).    
     Compute (execution [Ss 1 ; T 1 2] (1, reg0) 5).
     Compute (execution [Ss 1 ; T 1 2; J 1 1 1] (1, reg0) 5).    
-
-    Lemma exe1 : output Example2_1 (update_value (update_value reg0 1 9) 2 7) 12 = 2.
-     Proof. reflexivity. Qed.
-    Lemma exer2_2 : output Example2_1 (update_value (update_value (update_value reg0 1 8) 2 4) 3 2) 17 = 6.
-     Proof. reflexivity. Qed.
-    
-    Lemma never_stops_extension : forall n, forall in_reg, forall m, m<3 -> fst(execution [Ss 1;J 1 1 1] (m,in_reg) (n)) = false.
-     Proof. induction n.
-        -reflexivity.
-        -intros. simpl.
-        assert (self_eqb :forall n : nat, (n =? n) = true). {intros n0. apply Nat.eqb_eq. reflexivity. }
-        destruct m.
-        --simpl. apply IHn. lia.
-        -- destruct m.
-        --- 
-        (* inversion ths.  *)
-        simpl. apply IHn. lia.
-        --- destruct m.
-        ----simpl. rewrite self_eqb. apply IHn. lia.
-        ----lia.
-    Qed. 
-
-    Lemma never_stops : forall n, forall in_reg, fst(execution [Ss 1;J 1 1 1] (1,in_reg) (n)) = false.
-    Proof. intros. apply never_stops_extension. lia. Qed.
-        
-    Lemma exer2_3_extension :  forall n, forall in_reg, forall m, (in_reg 1 <? in_reg 2) = true -> m < 6 -> fst(snd(execution Example2_1 (m,in_reg) (n))) < 6.
-     Proof. induction n.
-        - simpl. lia.
-        -destruct m.
-        --intros. (*destruct H.*) simpl. destruct (in_reg 1 =? in_reg 2) eqn:ths.
-        +admit. 
-        +apply IHn. apply H. lia.
-        (* lia. rewrite H. rewrite H1. simpl. apply IHn. lia. lia. *)
-        -- destruct m.
-        --- simpl. intros. destruct (in_reg 1 =? in_reg 2) eqn:ths.
-        +admit.
-        +apply IHn. apply H. lia.
-         (* rewrite H. rewrite H1. apply IHn. lia. lia. *)
-        ---destruct m.
-        ----simpl. intros. specialize (IHn (update_value in_reg 2 (S (in_reg 2)))). apply IHn. unfold update_value. simpl.
-         admit. lia.
-        ----destruct m.
-        -----simpl. intros. specialize (IHn (update_value in_reg 3 (S (in_reg 3)))). apply IHn. unfold update_value. simpl.
-         apply H. lia.
-        -----destruct m.
-        +simpl. intros.  destruct (in_reg 1 =? in_reg 2) eqn:ths.
-        ++admit.
-        ++apply IHn. apply H. lia.
-        +destruct m.
-        +++intros. simpl. assert (self_eqb :forall n : nat, (n =? n) = true). {intros n0. apply Nat.eqb_eq. reflexivity. }
-        rewrite self_eqb. apply IHn. apply H. lia.
-        +++destruct m; intros; lia.
-    Admitted. (* Qed. *)
-
-    Lemma exer2_3: forall n, fst(snd(execution Example2_1 (1, (update_value (update_value reg0 1 2) 2 3)) (n))) < 6.
-     Proof. intros. eapply exer2_3_extension. unfold update_value. reflexivity. lia. Qed.
-
-    Lemma have_not_halted_means_did_not_halt : forall n, forall p, forall config, fst(execution p config (S n)) = false -> fst(execution p config n) = false.
-    Proof.
-    -Abort. (* couldn't find the right way to state the theorem *)
     
     
-    Definition ADD := [J 3 2 5;Ss 1;Ss 3;J 1 1 1].
-    Definition MINUS_ONE := [J 1 4 9;Ss 2;J 1 2 7; Ss 3;Ss 2;J 1 1 3;T 3 1].
-    Definition HALF_FOR_EVEN := [J 1 3 6;Ss 2;Ss 3;Ss 3;J 1 1 1;T 2 1].
-
-    Definition exer3_3_1a:= [J 1 2 4;Z 1;Ss 1].
-    Definition exer3_3_1b:= [Z 1;Ss 1;Ss 1;Ss 1;Ss 1;Ss 1].
-    Definition exer3_3_1c:= [J 1 2 5;Z 1;Ss 1;J 1 1 6;Z 1].
-    (* there's more exercises here *)
-
     Fixpoint standard_form_recursive (p: program) (length_p: nat) : program :=
     match p with
     |[] => []
@@ -181,7 +103,8 @@ Module URM.
     Compute standard_form [J 1 1 2].
     Compute standard_form [J 1 1 3;J 1 1 3].
 
-    Lemma standard_recursive_does_not_change_length : forall p:program, forall length_p: nat, length(p) = length(standard_form_recursive p length_p).
+    Lemma standard_recursive_does_not_change_length : forall p:program, forall length_p: nat,
+         length(p) = length(standard_form_recursive p length_p).
     Proof. intros. induction p.
         -reflexivity.
         -destruct a;try rewrite IHp;simpl; try (rewrite IHp; reflexivity).
@@ -193,87 +116,18 @@ Module URM.
     Qed.
 
 
-    Lemma standard_does_not_change_Zn_elements : forall command command':instruction, forall p: program, forall n m q k length_p: nat,
-    nth_error p k = Some command -> nth_error (standard_form_recursive p length_p) k = Some command'
-    -> (command = Z n -> command' = Z n).
-    Proof. 
-        intros command command' p n m q.
-        induction p.
-        -intros. destruct k;simpl in H;inversion H.
-        -intros k length_p. destruct k.
-        --intros. simpl in H. inversion H. rewrite H1 in H3. rewrite H3 in H0. simpl in H0. inversion H0. reflexivity.
-        --intros. simpl in H. destruct a;simpl in H0;specialize (IHp k length_p); try exact (IHp H H0 H1).
-        ---destruct (length_p <? q0);exact (IHp H H0 H1).
-    Qed. (* the rest cases are similar*)
-
-    Lemma standard_does_not_change_Ssn_elements : forall command command':instruction, forall p: program, forall n m q k length_p: nat,
-    nth_error p k = Some command -> nth_error (standard_form_recursive p length_p) k = Some command'
-    -> (command = Ss n -> command' = Ss n).
-    Proof. Admitted.
-    
-    Lemma standard_does_not_change_Tnm_elements : forall command command':instruction, forall p: program, forall n m q k length_p: nat,
-    nth_error p k = Some command -> nth_error (standard_form_recursive p length_p) k = Some command'
-    -> (command = T n m -> command' = T n m).
-    Proof. Admitted.
-    
-
-    Lemma standard_does_not_change_correct_Jnmq : forall command command': instruction, forall p: program, forall n m q k length_p,
-    nth_error p k = Some command -> nth_error (standard_form_recursive p length_p) k = Some command' -> (length_p <? q) = false
-    -> command = J n m q -> command' = J n m q.  
-    Proof.
-        intros command command' p n m q.
-        induction p.
-        -intros. destruct k;simpl in H;inversion H.
-        -intros. destruct k.
-        --intros. simpl in H. inversion H. rewrite H2 in H4. rewrite H4 in H0. simpl in H0.
-        rewrite H1 in H0. inversion H0. reflexivity.
-        --simpl in H. destruct a;try (simpl in H0;specialize (IHp k length_p);exact (IHp H H0 H1 H2)).
-        ---simpl in H0. destruct (length_p <? q0);simpl in H0;try (specialize (IHp k length_p);exact (IHp H H0 H1 H2)).
-    Qed.
-    (* the next proof is almost the same *)
-    Lemma standard_changes_Jnmq_correctly : forall command command': instruction, forall p: program, forall n m q k length_p,
-    nth_error p k = Some command -> nth_error (standard_form_recursive p length_p) k = Some command' -> (length_p <? q) = true
-    -> command = J n m q -> command' = J n m (length_p + 1).  
-    Proof.
-        intros command command' p n m q.
-        induction p.
-        -intros. destruct k;simpl in H;inversion H.
-        -intros. destruct k.
-        --intros. simpl in H. inversion H. rewrite H2 in H4. rewrite H4 in H0. simpl in H0.
-        rewrite H1 in H0. inversion H0. reflexivity.
-        --simpl in H. destruct a;try (simpl in H0;specialize (IHp k length_p);exact (IHp H H0 H1 H2)).
-        ---simpl in H0. destruct (length_p <? q0);simpl in H0;try (specialize (IHp k length_p);exact (IHp H H0 H1 H2)).
-    Qed.
-
-    Lemma standard_is_correct:  forall command command': instruction, forall p: program, forall n m q k length_p,
-    nth_error p k = Some command -> nth_error (standard_form_recursive p length_p) k = Some command'
-    ->(command = Z n -> command' = Z n) /\ (command = Ss n -> command' = Ss n)
-    /\ (command = T n m -> command' = T n m) /\ ((length_p <? q) = false -> command = J n m q -> command' = J n m q)
-    /\ ((length_p <? q) = true -> command = J n m q -> command' = J n m (length_p + 1)).
-    Proof. repeat split.
-        -eapply standard_does_not_change_Zn_elements; eauto.
-        -eapply standard_does_not_change_Ssn_elements; eauto.
-        -eapply standard_does_not_change_Tnm_elements; eauto.
-        -eapply standard_does_not_change_correct_Jnmq; eauto.
-        -eapply standard_changes_Jnmq_correctly; eauto.
-    Qed.
-
-
-
+    (* Join or concatenation of two programs *)
     Fixpoint Concat_recursive (Q : program) (length_p : nat) : program :=
     match Q with 
     | [] => []
     | J n m q :: Q' => J n m (q + (length_p)) :: Concat_recursive Q' length_p
     | h :: Q' => h :: Concat_recursive Q' length_p
     end.
-
     Definition Join (p q: program) : program := p ++ Concat_recursive q (length p).
         (* acts well whenever p is in its standard form*)
 
-    Lemma sth_about_join : forall p q,forall config, forall step,
-        execution (Join (standard_form p) q) config step = execution q (1, snd(snd(execution p config step))) step.
-    Proof. Abort. 
-    
+
+    (* Substitution *)
     Fixpoint ru_recursive (p : program) ( k : nat) : nat :=
     match p with 
     |[] => k
@@ -312,12 +166,12 @@ Module URM.
     end.
     Compute Clear_from_thisToThat 5 (12-5+1) 1.
 
-
-    (* move_and_compute := move_it_from_thisToThat_to_first_then_compute_and_put_output_there*)
+    
+    (* move_and_compute G n m l := G[n,...,m -> l] as defined in the book
+       (with this difference that registers in the left side are chosen sequentially here)*)
     Definition move_and_compute (p: program) (n m l: nat): program :=
     (move_it_from_thisToThat_to_first n (m-n+1) 1) ++ (Clear_from_thisToThat (n+1) (ru p - (n+1)) 1 ) ++ p ++ [T 1 l].
     Compute move_and_compute [Ss 5; T 6 4] 5 7 11.
-
 
     Fixpoint m_combine ( max_f : nat ) (P : list program): nat := 
     match P with 
@@ -344,44 +198,20 @@ Module URM.
 
     Definition Combine (f : program) (P : list program) ( n : nat): program := (* every p in P has n inputs *)
         neat_Combine f P n (m_combine (max n (max (length P) (ru f))) P) (length P).
-
     Compute Combine Identity_function [[Ss 1]] 1.
 
-    
-    Fixpoint re_list lst :=
-    match lst with 
-    |[] => []
-    |n :: t => Projection_function n :: re_list t
-    end.
-    Definition perrutation f per := Combine f (re_list per) (length per).
-    
-    (* Example 3.3*)
-    Fixpoint combine_repeat m (f: program) P n : program :=
-    match m with
-    |O => Combine f P n
-    |S m' => combine_repeat m' (Combine f P n) P n
-    end.
-    Definition constant x:= if x =? 0 then [Z 1] else (combine_repeat (x-1) Identity_function [[Ss 1]] 1).
-    Compute constant 1.
-    Compute output (constant 0) reg0 1000.
 
-
-    Example constant_function : forall m n x: nat, forall config:state, snd(snd (execution (Join [Z 1] (combine_repeat m Identity_function [[Ss 1]] 1)) config n)) 1= m.
-    Proof. -Abort.
-
+    (* Recursion *)
     Definition m_recusion f g n := max (n+2) (max (ru f) (ru g)).
-    Definition neat_recursion f g n m t q p := (transfer_x_to_m (n+1) m 1) ++ [T (t+1) (t+3);Z (t+1)] ++ (move_and_compute f 1 (n+1) (t+2)) ++ [J (t+1) (t+3) p] ++ (move_and_compute g (m+1) (m+n+2) (t+2)) ++ [Ss (t+1)] ++ [J 1 1 q;T (t+2) 1] .
-    Definition recursion f g n := neat_recursion f g n (m_recusion f g n) ((m_recusion f g n)+n) (n+1+2+(length (move_and_compute f 1 (n+1) ((m_recusion f g n)+n+2)))+1) (n+1+2+(length (move_and_compute f 1 (n+1) (((m_recusion f g n)+n)+2)))+1+(length (move_and_compute g ((m_recusion f g n)+1) ((m_recusion f g n)+n+2) (((m_recusion f g n)+n)+2)))+3).
     
-    Definition cut_off_by_one := recursion Zero_function (Projection_function 2) 1.
-    Compute cut_off_by_one.
-    Compute output cut_off_by_one (update_value reg0 2 10) 100.
-    (* Theorem 4.5 and others *)
-    (* bounded universal and existential quantifier can be sirulated by recursion*) 
+    Definition neat_recursion f g n m t q p := 
+    (transfer_x_to_m (n+1) m 1) ++ [T (t+1) (t+3);Z (t+1)] ++ (move_and_compute f 1 (n+1) (t+2))
+    ++ [J (t+1) (t+3) p] ++ (move_and_compute g (m+1) (m+n+2) (t+2)) ++ [Ss (t+1)] ++ [J 1 1 q;T (t+2) 1].
+    
+    Definition recursion f g n := neat_recursion f g n (m_recusion f g n) ((m_recusion f g n)+n) (n+1+2+(length (move_and_compute f 1 (n+1) ((m_recusion f g n)+n+2)))+1) (n+1+2+(length (move_and_compute f 1 (n+1) (((m_recusion f g n)+n)+2)))+1+(length (move_and_compute g ((m_recusion f g n)+1) ((m_recusion f g n)+n+2) (((m_recusion f g n)+n)+2)))+3).
 
-    Definition neat_minimalization f n m p q := (transfer_x_to_m (n) m 1) ++ (move_and_compute f (m+1) (m+n+1) 1) ++ [J 1 (m+n+2) q;Ss (m+n+1);J 1 1 p;T (m+n+1) 1].
-    Definition minimalization f n := neat_minimalization f n (max (n+1) (ru f)) (n+1) (n+(length (move_and_compute f ((max (n+1) (ru f))+1) ((max (n+1) (ru f))+n+1) 1))+4).
-    (* exercise 5.4 *)
-
-
-End URM.
+    (* Minimalisation *)
+    Definition neat_minimalisation f n m p q := 
+        (transfer_x_to_m (n) m 1) ++ (move_and_compute f (m+1) (m+n+1) 1) ++ [J 1 (m+n+2) q;Ss (m+n+1);J 1 1 p;T (m+n+1) 1].
+        
+    Definition minimalisation f n := neat_minimalisation f n (max (n+1) (ru f)) (n+1) (n+(length (move_and_compute f ((max (n+1) (ru f))+1) ((max (n+1) (ru f))+n+1) 1))+4).
